eliminate other single-letter variable names

chapter05/exercises/exercise01.dfy
@@ -1,6 +1,12 @@
 module Types {
   // TODO finite domain of keys so we can use finite-domained maps and avoid manager nonsense
   type Key(==, !new)
+
+  // Assume a finite domain (set is finite) of possible keys, so we
+  // can use (finite) maps. Dafny also offers infinite maps, but those
+  // bring another twist, so let's just use what's familiar for now.
+  function AllKeys() : set<Key>
+
   type Value(==, !new)
     // (==) means whatever this type is, it has equality defined on it.
     // !new means this type can't be allocated on the heap; it's a mathematical
@@ -12,38 +18,43 @@ module Types {
 
   function DefaultValue() : Value
     // No body -> this is an axiom.
+
+  function InitialMap() : map<Key, Value>
+  {
+    map key | key in AllKeys() :: DefaultValue()
+  }
 }
 
 module MapSpec {
   import opened Types
 
-  datatype Variables = Variables(m:map<Key, Value>)
+  datatype Variables = Variables(mapp:map<Key, Value>)
 
   predicate Init(v_: Variables)
   {
-    v_.m == map[]
+    v_.mapp == InitialMap()
   }
 
-  predicate InsertOp(v_:Variables, v_':Variables, k:Key, value:Value)
+  predicate InsertOp(v_:Variables, v_':Variables, key:Key, value:Value)
   {
-    v_'.m == v_.m[k := value]
+    v_'.mapp == v_.mapp[key := value]
   }
 
-  predicate QueryOp(v_:Variables, v_':Variables, k:Key, output:Value)
+  predicate QueryOp(v_:Variables, v_':Variables, key:Key, output:Value)
   {
-    && (output == if k in v_.m then v_.m[k] else DefaultValue())
+    && (output == if key in v_.mapp then v_.mapp[key] else DefaultValue())
     && v_' == v_  // no change to map state
   }
 
   datatype Step =
-    | InsertOpStep(k:Key, value:Value)
-    | QueryOpStep(k:Key, output:Value)
+    | InsertOpStep(key:Key, value:Value)
+    | QueryOpStep(key:Key, output:Value)
 
   predicate NextStep(v_: Variables, v_': Variables, step:Step)
   {
     match step
-      case InsertOpStep(k, value) => InsertOp(v_, v_', k, value)
-      case QueryOpStep(k, output) => QueryOp(v_, v_', k, output)
+      case InsertOpStep(key, value) => InsertOp(v_, v_', key, value)
+      case QueryOpStep(key, output) => QueryOp(v_, v_', key, output)
   }
 
   predicate Next(v_: Variables, v_': Variables)
@@ -58,50 +69,38 @@ module MapSpec {
 module Host {
   import opened Types
 
-  datatype Constants = Constants(manager: bool)
-  datatype Variables = Variables(m:map<Key, Value>)
+  datatype Constants = Constants()
+  datatype Variables = Variables(mapp:map<Key, Value>)
     // if a key is absent, only the manager can spring it
     // into existence.
 
-  predicate Init(c_: Constants, v_: Variables, i: nat)
+  predicate Init(c_: Constants, v_: Variables, hostidx: nat)
   {
-    && c_.manager == (i==0)
-    && v_.m == map[]
+    && v_.mapp == if hostidx==0 then InitialMap() else map[]
   }
 
-  predicate Insert(c_: Constants, v_: Variables, v_': Variables, k: Key, value: Value)
+  predicate Insert(c_: Constants, v_: Variables, v_': Variables, key: Key, value: Value)
   {
-    && k in v_.m // this host needs to be authoritative on this key
-    && v_'.m == v_.m[k := value]
+    && key in v_.mapp // this host needs to be authoritative on this key
+    && v_'.mapp == v_.mapp[key := value]
   }
 
-  predicate Query(c_: Constants, v_: Variables, v_': Variables, k: Key, output: Value)
+  predicate Query(c_: Constants, v_: Variables, v_': Variables, key: Key, output: Value)
   {
-    && k in v_.m
-    && output == v_.m[k]
+    && key in v_.mapp
+    && output == v_.mapp[key]
     && v_' == v_  // UNCHANGED
   }
 
-  // This is how we allow other hosts to serve queries for missing
-  // keys: we insert an explicit value to get the key into our map.
-  predicate FillDefault(c_: Constants, v_: Variables, v_': Variables, k: Key)
-  {
-    && c_.manager  // only manager is authoritative on missing keys
-    && k !in v_.m
-    && v_'.m == v_.m[k := DefaultValue()]
-  }
-
   datatype Step =
-    | InsertStep(k: Key, value: Value)
-    | QueryStep(k: Key, output: Value)
-    | FillDefaultStep(k: Key)
+    | InsertStep(key: Key, value: Value)
+    | QueryStep(key: Key, output: Value)
 
   predicate LocalOpStep(c_: Constants, v_: Variables, v_': Variables, step: Step)
   {
     match step
       case InsertStep(key, value) => Insert(c_, v_, v_', key, value)
       case QueryStep(key, output) => Query(c_, v_, v_', key, output)
-      case FillDefaultStep(key) => FillDefault(c_, v_, v_', key)
   }
 
   predicate LocalOp(c_: Constants, v_: Variables, v_': Variables)
@@ -109,21 +108,23 @@ module Host {
     exists step :: LocalOpStep(c_, v_, v_', step)
   }
 
-  datatype Message = TransferKey(k: Key, value: Value)
+  // A possible enhancement exercise: transfer many key,value pairs in one
+  // message.
+  datatype Message = TransferKey(key: Key, value: Value)
 
   // System-partial-actions for message transmission.
   // A matched pair of these happen together atomically, so it's a
   // "synchronous" message delivery model. (We'll add more realism later.)
   predicate Send(c_: Constants, v_: Variables, v_': Variables, msg: Message)
   {
-    && msg.k in v_.m // can only give away what I'm authoritative for
-    && v_.m[msg.k] == msg.value  // transmit the correct value
-    && v_'.m == map k | k in v_.m && k!=msg.k :: v_.m[k] // forget this key
+    && msg.key in v_.mapp // can only give away what I'mapp authoritative for
+    && v_.mapp[msg.key] == msg.value  // transmit the correct value
+    && v_'.mapp == map key | key in v_.mapp && key!=msg.key :: v_.mapp[key] // forget this key
   }
 
   predicate Receive(c_: Constants, v_: Variables, v_': Variables, msg: Message)
   {
-    && v_'.m == v_.m[msg.k := msg.value]  // learn the new key,value pair.
+    && v_'.mapp == v_.mapp[msg.key := msg.value]  // learn the new key,value pair.
   }
 }
 
@@ -132,7 +133,8 @@ module System {
 
   datatype Constants = Constants(hosts: seq<Host.Constants>)
   {
-    predicate ValidHost(i: nat) { i < |hosts| }
+    predicate WF() { 0 < |hosts| }
+    predicate ValidHost(hostidx: nat) { hostidx < |hosts| }
   }
 
   datatype Variables = Variables(hosts: seq<Host.Variables>)
@@ -142,18 +144,19 @@ module System {
   
   predicate Init(c_: Constants, v_: Variables)
   {
+    && c_.WF()
     && v_.WF(c_)
-    && (forall i:nat | c_.ValidHost(i) :: Host.Init(c_.hosts[i], v_.hosts[i], i))
+    && (forall hostidx:nat | c_.ValidHost(hostidx) :: Host.Init(c_.hosts[hostidx], v_.hosts[hostidx], hostidx))
   }
 
-  predicate LocalOp(c_: Constants, v_: Variables, v_': Variables, i: nat)
+  predicate LocalOp(c_: Constants, v_: Variables, v_': Variables, hostidx: nat)
   {
     && v_.WF(c_)
     && v_'.WF(c_)
-    && c_.ValidHost(i)
-    && Host.LocalOp(c_.hosts[i], v_.hosts[i], v_'.hosts[i])
+    && c_.ValidHost(hostidx)
+    && Host.LocalOp(c_.hosts[hostidx], v_.hosts[hostidx], v_'.hosts[hostidx])
     // all other host state UNCHANGED
-    && (forall j:nat | c_.ValidHost(j) && j!=i :: v_'.hosts[j] == v_.hosts[j])
+    && (forall otherhost:nat | c_.ValidHost(otherhost) && otherhost!=hostidx :: v_'.hosts[otherhost] == v_.hosts[otherhost])
   }
 
   predicate TransmitOp(c_: Constants, v_: Variables, v_': Variables, src: nat, dst: nat, message: Host.Message)
@@ -165,18 +168,18 @@ module System {
     && Host.Send(c_.hosts[src], v_.hosts[src], v_'.hosts[src], message)
     && Host.Receive(c_.hosts[dst], v_.hosts[dst], v_'.hosts[dst], message)
     // all other host state UNCHANGED
-    && (forall j:nat | c_.ValidHost(j) && j!=src && j!=dst
-        :: v_'.hosts[j] == v_.hosts[j])
+    && (forall otherhost:nat | c_.ValidHost(otherhost) && otherhost!=src && otherhost!=dst
+        :: v_'.hosts[otherhost] == v_.hosts[otherhost])
   }
 
   datatype Step =
-    | LocalOpStep(i:nat)
+    | LocalOpStep(hostidx:nat)
     | TransmitOpStep(src:nat, dst:nat, message:Host.Message)
 
   predicate NextStep(c_: Constants, v_: Variables, v_': Variables, step:Step)
   {
     match step
-      case LocalOpStep(i) => LocalOp(c_, v_, v_', i)
+      case LocalOpStep(hostidx) => LocalOp(c_, v_, v_', hostidx)
       case TransmitOpStep(src, dst, message) => TransmitOp(c_, v_, v_', src, dst, message)
   }
 
@@ -191,23 +194,23 @@ module RefinementProof {
   import MapSpec
   import opened System
 
-  predicate HostHasKey(c_: Constants, v_: Variables, i:nat, k:Key)
+  predicate HostHasKey(c_: Constants, v_: Variables, hostidx:nat, key:Key)
     requires v_.WF(c_)
   {
-    && c_.ValidHost(i)
-    && k in v_.hosts[i].m
+    && c_.ValidHost(hostidx)
+    && key in v_.hosts[hostidx].mapp
   }
 
   // Pulling the choose out into its own function is sometimes necessary due
   // to a (deliberate) stupidity in Dafny: it doesn't treat :| expressions
   // as subsitution-equivalent, even though the are (as evidenced by pulling
   // one into a function).
-  function TheHostWithKey(c_: Constants, v_: Variables, k:Key) : nat
+  function TheHostWithKey(c_: Constants, v_: Variables, key:Key) : nat
     requires v_.WF(c_)
-    requires exists i :: HostHasKey(c_, v_, i, k);
+    requires exists hostidx :: HostHasKey(c_, v_, hostidx, key);
   {
-    var i:nat :| HostHasKey(c_, v_, i, k);
-    i
+    var hostidx:nat :| HostHasKey(c_, v_, hostidx, key);
+    hostidx
   }
 
 
@@ -216,7 +219,7 @@ module RefinementProof {
   {
     if exists idx :: HostHasKey(c_, v_, idx, key)
     then
-      v_.hosts[TheHostWithKey(c_, v_, key)].m[key]
+      v_.hosts[TheHostWithKey(c_, v_, key)].mapp[key]
     else DefaultValue()
   }
 
@@ -229,7 +232,7 @@ module RefinementProof {
     requires v_.WF(c_)
     requires count <= |c_.hosts|
   {
-    if count==0 then {} else AllKeysRecurse(c_, v_, count-1) + v_.hosts[count-1].m.Keys
+    if count==0 then {} else AllKeysRecurse(c_, v_, count-1) + v_.hosts[count-1].mapp.Keys
   }
 
   function AllKeys(c_: Constants, v_: Variables) : set<Key>
@@ -241,32 +244,39 @@ module RefinementProof {
   function Abstraction(c_: Constants, v_: Variables) : MapSpec.Variables
     requires v_.WF(c_)
   {
-    MapSpec.Variables(map k | k in AllKeys(c_, v_) :: Ikey(c_, v_, k))
+    MapSpec.Variables(map key | key in AllKeys(c_, v_) :: Ikey(c_, v_, key))
   }
 
   predicate Inv(c_: Constants, v_: Variables)
   {
+    && c_.WF()
     && v_.WF(c_)
     // No two distinct hosts have the same key.
-    && (forall k, i:nat, j:nat
-        | && c_.ValidHost(i) && c_.ValidHost(j)
-          && k in v_.hosts[i].m && k in v_.hosts[j].m
-        :: i == j
+    && (forall key, hostidx:nat, otherhost:nat
+        | && c_.ValidHost(hostidx) && c_.ValidHost(otherhost)
+          && key in v_.hosts[hostidx].mapp && key in v_.hosts[otherhost].mapp
+        :: hostidx == otherhost
       )
   }
 
-//  lemma InitAllKeysEmpty(c_: Constants, v_: Variables, count: nat)
-//    requires Init(c_, v_)
-//    requires count <= |c_.hosts|
-//    ensures AllKeysRecurse(c_, v_, count) == {}
-//  {
-//  }
-//
+  lemma InitAllKeysEmpty(c_: Constants, v_: Variables, count: nat)
+    requires Init(c_, v_)
+    requires 0 < count <= |c_.hosts|
+    ensures AllKeysRecurse(c_, v_, count) == InitialMap().Keys
+  {
+    if count==1 {
+      assert AllKeysRecurse(c_, v_, count) == v_.hosts[0].mapp.Keys == InitialMap().Keys;
+    } else {
+      InitAllKeysEmpty(c_, v_, count-1);
+    }
+    
+  }
+
   lemma AllKeysMembership(c_: Constants, v_: Variables, count: nat)
     requires Inv(c_, v_)
     requires count <= |c_.hosts|
-    ensures forall k ::
-      (k in AllKeysRecurse(c_, v_, count) <==> exists i:nat :: i<count && k in v_.hosts[i].m)
+    ensures forall key ::
+      (key in AllKeysRecurse(c_, v_, count) <==> exists hostidx:nat :: hostidx<count && key in v_.hosts[hostidx].mapp)
   {
   }
 
@@ -275,7 +285,7 @@ module RefinementProof {
     ensures MapSpec.Init(Abstraction(c_, v_))
     ensures Inv(c_, v_)
   {
-   // InitAllKeysEmpty(c_, v_, |c_.hosts|);
+    InitAllKeysEmpty(c_, v_, |c_.hosts|);
     AllKeysMembership(c_, v_, |c_.hosts|);
   }
 
@@ -283,38 +293,38 @@ module RefinementProof {
     requires Inv(c_, v_)
     requires Next(c_, v_, v_')
     requires c_.ValidHost(insertHost)
-    requires (forall j:nat | c_.ValidHost(j) && j!=insertHost :: v_'.hosts[j] == v_.hosts[j]);
+    requires (forall otherhost:nat | c_.ValidHost(otherhost) && otherhost!=insertHost :: v_'.hosts[otherhost] == v_.hosts[otherhost]);
     requires Host.Insert(c_.hosts[insertHost], v_.hosts[insertHost], v_'.hosts[insertHost], insertedKey, value)
     ensures Inv(c_, v_')
     ensures MapSpec.Next(Abstraction(c_, v_), Abstraction(c_, v_'))
   {
-    var im := Abstraction(c_, v_).m;
-    var im' := Abstraction(c_, v_').m;
+    var im := Abstraction(c_, v_).mapp;
+    var im' := Abstraction(c_, v_').mapp;
 
-    forall k
-      ensures k in im' <==> k in im || k == insertedKey // domain
-      ensures k in im' ==> (im'[k] == if k==insertedKey then value else im[k])  // value
+    forall key
+      ensures key in im' <==> key in im || key == insertedKey // domain
+      ensures key in im' ==> (im'[key] == if key==insertedKey then value else im[key])  // value
     {
       AllKeysMembership(c_, v_', |c_.hosts|);
       // Narrowing the calls to AllKeysMembership(v_) helps z3 save 15s!
       // (But domain proof can be replaced with just AllKeysMembership(v_);AllKeysMembership(v_') and it'll still work.)
-      if k == insertedKey {
-      } else if k in im' {
-        assert k in im by { AllKeysMembership(c_, v_, |c_.hosts|); }
-      } else if k in im {
-        assert k in im' by { AllKeysMembership(c_, v_, |c_.hosts|); }
+      if key == insertedKey {
+      } else if key in im' {
+        assert key in im by { AllKeysMembership(c_, v_, |c_.hosts|); }
+      } else if key in im {
+        assert key in im' by { AllKeysMembership(c_, v_, |c_.hosts|); }
       }
 
-      if k in im' {
-        if k==insertedKey {
-          assert HostHasKey(c_, v_', insertHost, k);  // trigger
-          assert Ikey(c_, v_', k) == value; // trigger
+      if key in im' {
+        if key==insertedKey {
+          assert HostHasKey(c_, v_', insertHost, key);  // trigger
+          assert Ikey(c_, v_', key) == value; // trigger
         } else {
-          var ihost:nat :| ihost<|c_.hosts| && k in v_'.hosts[ihost].m;
-          assert forall j | c_.ValidHost(j) && j!=ihost :: !HostHasKey(c_, v_, j, k);  // trigger
-          assert HostHasKey(c_, v_', ihost, k) by { AllKeysMembership(c_, v_, |c_.hosts|); }
-          assert TheHostWithKey(c_, v_', k) == ihost; // witness
-          assert im'[k] == im[k]; // trigger
+          var ihost:nat :| ihost<|c_.hosts| && key in v_'.hosts[ihost].mapp;
+          assert forall otherhost | c_.ValidHost(otherhost) && otherhost!=ihost :: !HostHasKey(c_, v_, otherhost, key);  // trigger
+          assert HostHasKey(c_, v_', ihost, key) by { AllKeysMembership(c_, v_, |c_.hosts|); }
+          assert TheHostWithKey(c_, v_', key) == ihost; // witness
+          assert im'[key] == im[key]; // trigger  // TODO unstable?
         }
       }
     }
@@ -334,17 +344,12 @@ module RefinementProof {
       case LocalOpStep(idx) => {
         var hstep :| Host.LocalOpStep(c_.hosts[idx], v_.hosts[idx], v_'.hosts[idx], hstep);
         match hstep
-          case InsertStep(k, value) => InsertPreservesInvAndRefines(c_, v_, v_', idx, k, value);
-          case QueryStep(k, output) => {
-            assume false;
+          case InsertStep(key, value) => InsertPreservesInvAndRefines(c_, v_, v_', idx, key, value);
+          case QueryStep(key, output) => {
             assert Inv(c_, v_');
+            assert v_ == v_'; // weirdly obvious trigger
             assert Abstraction(c_, v_) == Abstraction(c_, v_');
-            assert MapSpec.Next(Abstraction(c_, v_), Abstraction(c_, v_'));
-          }
-          case FillDefaultStep(k) => {
-            assume false;
-            assert Inv(c_, v_');
-            assert Abstraction(c_, v_) == Abstraction(c_, v_');
+            assert MapSpec.NextStep(Abstraction(c_, v_), Abstraction(c_, v_'), MapSpec.QueryOpStep(key, output));
             assert MapSpec.Next(Abstraction(c_, v_), Abstraction(c_, v_'));
           }
       }
